\documentclass[12pt]{article}
\usepackage{pmmeta}
\pmcanonicalname{abcdIfAndOnlyIfAcAndBd}
\pmcreated{2013-03-22 16:13:19}
\pmmodified{2013-03-22 16:13:19}
\pmowner{Wkbj79}{1863}
\pmmodifier{Wkbj79}{1863}
\pmtitle{$(a,b)=(c,d)$ if and only if $a=c$ and $b=d$}
\pmrecord{9}{38320}
\pmprivacy{1}
\pmauthor{Wkbj79}{1863}
\pmtype{Proof}
\pmcomment{trigger rebuild}
\pmclassification{msc}{03-00}

\usepackage{amssymb}
\usepackage{amsmath}
\usepackage{amsfonts}

\usepackage{psfrag}
\usepackage{graphicx}
\usepackage{amsthm}
%%\usepackage{xypic}

\begin{document}
Following is a proof that the ordered pairs $(a,b)$ and $(c,d)$ are equal if and only if $a=c$ and $b=d$.

\begin{proof}
If $a=c$ and $b=d$, then $(a,b)=\{\{a\},\{a,b\}\}=\{\{c\},\{c,d\}\}=(c,d)$.

Assume that $(a,b)=(c,d)$ and $a=b$.  Then $\{\{c\},\{c,d\}\}=(c,d)=(a,b)=\{\{a\},\{a,b\}\}=\{\{a\},\{a,a\}\}=\{\{a\},\{a\}\}=\{\{a\}\}$.
Thus, $\{c,d\}\in\{\{a\}\}$.  Therefore, $\{c,d\}=\{a\}$.  Hence, $a=c$ and $a=d$.  Since it was also assumed that $a=b$, it follows that $a=c$ and $b=d$.

Finally, assume that $(a,b)=(c,d)$ and $a \neq b$.  Then $\{a\} \neq \{a,b\}$.  Note that $\{\{a\},\{a,b\}\}=(a,b)=(c,d)=\{\{c\},\{c,d\}\}$.  Thus, $\{c\} \in \{\{a\},\{a,b\}\}$.  It cannot be the case that $\{c\}=\{a,b\}$ (lest $a=c=b$).  Thus, $\{c\}=\{a\}$.  Therefore, $a=c$.  Hence, $\{\{a\},\{a,b\}\}=\{\{c\},\{c,d\}\}=\{\{a\},\{a,d\}\}$.  Note that $\{a,b\} \in \{\{a\},\{a,d\}\}$.  Since $\{a\} \neq \{a,b\}$, it must be the case that $\{a,b\}=\{a,d\}$.  Thus, $b \in \{a,d\}$.  Since $a \neq b$, it must be the case that $b=d$.  It follows that $a=c$ and $b=d$.
\end{proof}
%%%%%
%%%%%
\end{document}
